# baseURI: http://pid.geoscience.gov.au/def/stratname
# imports: file:///C:/Users/cox075/dev/cache-external/schema.ttl
# imports: https://linked.data.gov.au/def/geox
# imports: http://purl.org/dc/elements/1.1/
# imports: http://resource.geosciml.org/ontology/timescale/gts
# imports: http://www.opengis.net/ont/geosparql
# imports: http://www.w3.org/ns/prov-o#
# prefix: strat

@prefix dcterms: <http://purl.org/dc/terms/> .
@prefix geo: <http://www.opengis.net/ont/geosparql#> .
@prefix lith: <http://pid.geoscience.gov.au/def/stratname/lithology/> .
@prefix owl: <http://www.w3.org/2002/07/owl#> .
@prefix proc: <http://pid.geoscience.gov.au/def/stratname/process/> .
@prefix rdf: <http://www.w3.org/1999/02/22-rdf-syntax-ns#> .
@prefix rdfs: <http://www.w3.org/2000/01/rdf-schema#> .
@prefix rel: <http://pid.geoscience.gov.au/def/stratname/relation/> .
@prefix schema: <http://schema.org/> .
@prefix sdo: <https://schema.org/> .
@prefix skos: <http://www.w3.org/2004/02/skos/core#> .
@prefix strat: <http://pid.geoscience.gov.au/def/stratname#> .
@prefix xsd: <http://www.w3.org/2001/XMLSchema#> .

<http://pid.geoscience.gov.au/def/stratname>
  a owl:Ontology ;
  dcterms:created "2020-06-15"^^xsd:date ;
  dcterms:creator <https://orcid.org/0000-0002-3884-3420> ;
  dcterms:description """An ontology for the Australian Stratnames dataset, with preliminary alignment to the Geological Timescale Ontology. 

The ontology is based around the usual assumptions made in geological mapping - 
i.e. that the earth can be divided into 'units' that are distinguished from one another on lithological, chronological, geophysical, geochemical or other bases essentially connected with some aspect of their genesis. 

Stratigraphic units are distinguished primarily on the basis of having been formed by some relatively uniform geologic process (and thus be composed of a relatively uniform lithological material) during a discrete time interval. 
Note that any particular _occurence_ of a unit might not contain earth materials that cover the complete time span. 

In the GA Stratnames dataset, the timing of the base and top (i.e. the max and min age) are specified as geologic eras - i.e. time-intervals - which implies a degree of uncertainty or variation in the exact temporal position of the boundary. 
Variation may be due to the terminating event applying at different times in different places. 

![](../images/overview.png)""" ;
  dcterms:modified "2020-06-17"^^xsd:date ;
  dcterms:title "Stratnames ontology" ;
  schema:codeRepository <https://github.com/GeoscienceAustralia/strat-ontology-graph-API> ;
  rdfs:seeAlso <https://www.ga.gov.au/data-pubs/datastandards/stratigraphic-units> ;
  owl:imports <file:///C:/Users/cox075/dev/cache-external/schema.ttl> ;
  owl:imports <https://linked.data.gov.au/def/geox> ;
  owl:imports <http://purl.org/dc/elements/1.1/> ;
  owl:imports <http://resource.geosciml.org/ontology/timescale/gts> ;
  owl:imports <http://www.opengis.net/ont/geosparql> ;
  owl:imports <http://www.w3.org/ns/prov-o#> ;
.
strat:Boundary
  a owl:Class ;
  rdfs:label "Stratigraphic boundary"@en ;
  rdfs:subClassOf strat:Entity ;
  rdfs:subClassOf [
      a owl:Restriction ;
      owl:allValuesFrom strat:Point ;
      owl:onProperty strat:stratotype ;
    ] ;
.
strat:Entity
  a owl:Class ;
  rdfs:label "Stratigraphic entity"@en ;
  rdfs:subClassOf geo:Feature ;
  rdfs:subClassOf [
      a owl:Restriction ;
      owl:allValuesFrom <http://www.w3.org/ns/prov#Agent> ;
      owl:onProperty strat:wasDefinedBy ;
    ] ;
.
strat:Event
  a owl:Class ;
  rdfs:label "Geologic event" ;
  rdfs:subClassOf strat:Entity ;
.
strat:Geologic-process
  a owl:Class ;
  rdfs:label "Geological Process "@en ;
  rdfs:subClassOf skos:Concept ;
.
strat:Lithology-group
  a owl:Class ;
  rdfs:label "Lithology group"@en ;
  rdfs:subClassOf skos:Concept ;
.
strat:Point
  a owl:Class ;
  rdfs:comment "Point or level within a section through a continuous sequence of rocks (which may be representative of a stratigraphic boundary)"@en ;
  rdfs:label "Stratigraphic point"@en ;
  rdfs:subClassOf strat:Site ;
  rdfs:subClassOf [
      a owl:Restriction ;
      owl:onProperty strat:within ;
      owl:someValuesFrom strat:Section ;
    ] ;
.
strat:Province
  a owl:Class ;
  rdfs:label "Geologic province" ;
  rdfs:subClassOf strat:Entity ;
  rdfs:subClassOf [
      a owl:Restriction ;
      owl:cardinality "1"^^xsd:nonNegativeInteger ;
      owl:onProperty geo:hasGeometry ;
    ] ;
.
strat:Relation-type
  a owl:Class ;
  rdfs:label "Stratigraphic relation type"@en ;
  rdfs:subClassOf skos:Concept ;
.
strat:Relationship
  a owl:Class ;
  rdfs:label "Association class relating a geologic entity to another" ;
  rdfs:subClassOf <http://www.w3.org/ns/prov#EntityInfluence> ;
  rdfs:subClassOf [
      a owl:Restriction ;
      owl:cardinality "1"^^xsd:nonNegativeInteger ;
      owl:onProperty strat:context ;
    ] ;
  rdfs:subClassOf [
      a owl:Restriction ;
      owl:cardinality "1"^^xsd:nonNegativeInteger ;
      owl:onProperty strat:relation ;
    ] ;
  rdfs:subClassOf [
      a owl:Restriction ;
      owl:cardinality "1"^^xsd:nonNegativeInteger ;
      owl:onProperty strat:relationshipType ;
    ] ;
  skos:example """
stratnames:u10834overliesu488
  rdf:type strat:Relationship ;
  strat:context stratnames:u10834 ;
  strat:relation stratnames:u488 ;
  strat:relationshipType rel:overlies ;
.
""" ;
.
strat:Section
  a owl:Class ;
  rdfs:comment "Outcrop showing a continuous sequence of rocks (which may be representative of a stratigraphic unit)"@en ;
  rdfs:label "Stratigraphic section"@en ;
  rdfs:subClassOf strat:Site ;
.
strat:Site
  a owl:Class ;
  rdfs:label "Geological site "@en ;
  rdfs:subClassOf geo:Feature ;
.
strat:Unit
  a owl:Class ;
  rdfs:label "Stratigraphic unit"@en ;
  rdfs:subClassOf strat:Entity ;
  rdfs:subClassOf [
      a owl:Restriction ;
      owl:allValuesFrom strat:Section ;
      owl:onProperty strat:stratotype ;
    ] ;
  rdfs:subClassOf [
      a owl:Restriction ;
      owl:cardinality "1"^^xsd:nonNegativeInteger ;
      owl:onProperty dcterms:identifier ;
    ] ;
  rdfs:subClassOf [
      a owl:Restriction ;
      owl:cardinality "1"^^xsd:nonNegativeInteger ;
      owl:onProperty dcterms:title ;
    ] ;
  rdfs:subClassOf [
      a owl:Restriction ;
      owl:onProperty strat:relation ;
      owl:someValuesFrom strat:Province ;
    ] ;
  skos:example """
stratnames:u27732
  rdf:type strat:Unit ;
  strat:bottomAge <http://resource.geosciml.org/classifier/ics/ischart/Pliocene> ;
  strat:formationProcess proc:deposition ;
  strat:lithology lith:medium-coarse_grained_siliciclastic_rock ;
  strat:qualifiedRelation [
      rdf:type strat:Relationship ;
      strat:relation stratnames:u24044 ;
      strat:relationshipType rel:underlies ;
    ] ;
  strat:relation stratnames:p20430 ;
  strat:terminationProcess proc:deposition ;
  strat:topAge <http://resource.geosciml.org/classifier/ics/ischart/Pleistocene> ;
  strat:wasDefinedBy <https://orcid.org/0000-1111-2222-3333> ;
  dct:identifier \"27732\" ;
  dct:title \"Campaspe Formation\" ;
  rdfs:label \"Campaspe Formation\" ;
.
""" ;
.
strat:age
  a owl:ObjectProperty ;
  dcterms:description "age of stratigraphic entity"@en ;
  rdfs:comment "age of stratigraphic entity"@en ;
  rdfs:domain strat:Entity ;
  rdfs:label "has age"@en ;
  rdfs:subPropertyOf <http://www.w3.org/2006/time#hasTime> ;
.
strat:bottom
  a owl:ObjectProperty ;
  dcterms:description "Boundary of base of unit"@en ;
  rdfs:comment "Boundary of base of unit"@en ;
  rdfs:domain strat:Unit ;
  rdfs:label "bottom boundary"@en ;
  rdfs:range strat:Boundary ;
  rdfs:subPropertyOf strat:relation ;
.
strat:bottomAge
  a owl:ObjectProperty ;
  dcterms:description "Age of base of unit"@en ;
  rdfs:comment "Age of base of unit"@en ;
  rdfs:domain strat:Unit ;
  rdfs:label "Age of base"@en ;
  rdfs:subPropertyOf <http://www.w3.org/2006/time#hasTime> ;
  owl:propertyChainAxiom (
      strat:bottom
      strat:age
    ) ;
  skos:example """
stratnames:u27732
  rdf:type strat:Unit ;
  strat:bottomAge <http://resource.geosciml.org/classifier/ics/ischart/Pliocene> ;
.
""" ;
.
strat:contains
  a owl:ObjectProperty ;
  rdfs:label "contains"@en ;
  rdfs:subPropertyOf dcterms:relation ;
.
strat:context
  a owl:ObjectProperty ;
  rdfs:comment "the context of the relationship" ;
  rdfs:domain strat:Relationship ;
  rdfs:label "context" ;
  rdfs:range strat:Entity ;
.
strat:correlatesWith
  a owl:ObjectProperty ;
  dcterms:description "This property points from a geologic feature or event to a geochronologic element"@en ;
  rdfs:comment "This property points from a geologic feature or event to a geochronologic element"@en ;
  rdfs:label "correlating boundary or era" ;
  rdfs:range [
      a owl:Class ;
      owl:unionOf (
          <http://resource.geosciml.org/ontology/timescale/gts#GeochronologicBoundary>
          <http://resource.geosciml.org/ontology/timescale/gts#GeochronologicEra>
        ) ;
    ] ;
.
strat:formationProcess
  a owl:ObjectProperty ;
  dcterms:description "Process that formed the geologic entity"@en ;
  rdfs:comment "Process that formed the geologic entity"@en ;
  rdfs:domain strat:Entity ;
  rdfs:label "formation process"@en ;
  rdfs:range strat:Geologic-process ;
  skos:example """
stratnames:u27732
  rdf:type strat:Unit ;
  strat:formationProcess proc:deposition ;
.
""" ;
.
strat:holostratotype
  a owl:ObjectProperty ;
  dcterms:description "the original stratotype designated by the original author at the time of proposing a stratigraphic unit or boundary"@en ;
  rdfs:comment "the original stratotype designated by the original author at the time of proposing a stratigraphic unit or boundary"@en ;
  rdfs:label "holostratotype"@en ;
  rdfs:subPropertyOf strat:stratotype ;
.
strat:hypostratotype
  a owl:ObjectProperty ;
  dcterms:description "a stratotype proposed after the original designation of the holostratotype (and parastratotype) in order to extend knowledge of the unit or boundary to other geographic areas. It is always subordinate to the holostratotype"@en ;
  rdfs:comment "a stratotype proposed after the original designation of the holostratotype (and parastratotype) in order to extend knowledge of the unit or boundary to other geographic areas. It is always subordinate to the holostratotype"@en ;
  rdfs:label "hypostratotype"@en ;
  rdfs:subPropertyOf strat:stratotype ;
.
strat:initiationProcess
  a owl:ObjectProperty ;
  dcterms:description "Process that initiated the geologic entity"@en ;
  rdfs:comment "Process that initiated the geologic entity"@en ;
  rdfs:domain strat:Entity ;
  rdfs:label "initiation process"@en ;
  rdfs:range strat:Geologic-process ;
.
strat:lectostratotype
  a owl:ObjectProperty ;
  dcterms:description "a stratotype for a previously described stratigraphic unit selected later in the absence of an adequately designated original stratotype (holostratotype)"@en ;
  rdfs:comment "a stratotype for a previously described stratigraphic unit selected later in the absence of an adequately designated original stratotype (holostratotype)"@en ;
  rdfs:label "lectostratotype"@en ;
  rdfs:subPropertyOf strat:stratotype ;
.
strat:lithology
  a owl:ObjectProperty ;
  dcterms:description "Characteristic lithological material for the geologic entity"@en ;
  rdfs:comment "Characteristic lithological material for the geologic entity"@en ;
  rdfs:domain strat:Unit ;
  rdfs:label "characteristic lithology"@en ;
  rdfs:range strat:Lithology-group ;
  skos:example """
stratnames:u27732
  rdf:type strat:Unit ;
  strat:lithology lith:medium-coarse_grained_siliciclastic_rock ;
.
""" ;
.
strat:manifestedBy
  a owl:ObjectProperty ;
  dcterms:description "This property points from a geochronologic element to a geologic feature which shows characteristics associated with the event associated with the boundary or era"@en ;
  rdfs:comment "This property points from a geochronologic element to a geologic feature which shows characteristics associated with the event associated with the boundary or era"@en ;
  rdfs:domain [
      a owl:Class ;
      owl:unionOf (
          <http://resource.geosciml.org/ontology/timescale/gts#GeochronologicBoundary>
          <http://resource.geosciml.org/ontology/timescale/gts#GeochronologicEra>
        ) ;
    ] ;
  rdfs:label "geologic manifestation" ;
  owl:inverseOf strat:correlatesWith ;
.
strat:neostratotype
  a owl:ObjectProperty ;
  dcterms:description "a new stratotype selected to replace an older one which has been destroyed, covered, or otherwise made inaccessible"@en ;
  rdfs:comment "a new stratotype selected to replace an older one which has been destroyed, covered, or otherwise made inaccessible"@en ;
  rdfs:label "neostratotype"@en ;
  rdfs:subPropertyOf strat:stratotype ;
.
strat:parastratotype
  a owl:ObjectProperty ;
  dcterms:description "a supplementary stratotype used in the original definition by the original author to illustrate the diversity or heterogeneity of the defined stratigraphic unit or some critical feature not evident or exposed in the holostratotype"@en ;
  rdfs:comment "a supplementary stratotype used in the original definition by the original author to illustrate the diversity or heterogeneity of the defined stratigraphic unit or some critical feature not evident or exposed in the holostratotype"@en ;
  rdfs:label "parastratotype"@en ;
  rdfs:subPropertyOf strat:stratotype ;
.
strat:qualifiedRelation
  a owl:ObjectProperty ;
  dcterms:description "Association to another geologic unit"@en ;
  rdfs:comment "Association to another geologic unit"@en ;
  rdfs:domain strat:Entity ;
  rdfs:label "qualified relation" ;
  rdfs:range strat:Relationship ;
  skos:example """
stratnames:u27732
  rdf:type strat:Unit ;
  strat:qualifiedRelation [
      rdf:type strat:Relationship ;
      strat:relation stratnames:u24044 ;
      strat:relationshipType rel:underlies ;
    ] ;
.
""" ;
.
strat:relation
  a owl:ObjectProperty ;
  dcterms:description "The related geologic entity"@en ;
  rdfs:comment "The related geologic entity"@en ;
  rdfs:label "relation" ;
  rdfs:range strat:Entity ;
  rdfs:subPropertyOf dcterms:relation ;
  skos:example """
stratnames:u27732
  rdf:type strat:Unit ;
  strat:qualifiedRelation [
      rdf:type strat:Relationship ;
      strat:relation stratnames:u24044 ;
      strat:relationshipType rel:underlies ;
    ] ;
  strat:relation stratnames:p20430 ;
.
""" ;
.
strat:relationshipType
  a owl:ObjectProperty ;
  dcterms:description "The nature of the relationship between two geologic entities"@en ;
  rdfs:comment "The nature of the relationship between two geologic entities"@en ;
  rdfs:domain strat:Relationship ;
  rdfs:label "has relationship type"@en ;
  rdfs:range strat:Relation-type ;
  skos:example """
stratnames:u27732
  rdf:type strat:Unit ;
  strat:qualifiedRelation [
      rdf:type strat:Relationship ;
      strat:relation stratnames:u24044 ;
      strat:relationshipType rel:underlies ;
    ] ;
.
""" ;
.
strat:stratotype
  a owl:ObjectProperty ;
  dcterms:description "type manifestation of the stratigraphic entity: section for a unit; point or surface for a boundary or event"@en ;
  dcterms:source "Salvador, A (Editor) 1994, International Stratigraphic Guide: A guide to stratigraphic classification, terminology, and procedure. 2nd edition. International Union of Geological Sciences and the Geological Society of America, Boulder, Colorado." ;
  rdfs:comment "type manifestation of the stratigraphic entity: section for a unit; point or surface for a boundary or event"@en ;
  rdfs:domain strat:Entity ;
  rdfs:label "stratotype"@en ;
  rdfs:range strat:Site ;
  rdfs:seeAlso <https://www.ga.gov.au/data-pubs/datastandards/stratigraphic-units/stratotypes> ;
  rdfs:subPropertyOf strat:manifestedBy ;
.
strat:terminationProcess
  a owl:ObjectProperty ;
  dcterms:description "Process that terminated the formation of the geologic entity"@en ;
  rdfs:comment "Process that terminated the formation of the geologic entity"@en ;
  rdfs:domain strat:Entity ;
  rdfs:label "termination process"@en ;
  rdfs:range strat:Geologic-process ;
  skos:example """
stratnames:u27732
  rdf:type strat:Unit ;
  strat:terminationProcess proc:deposition ;
.
""" ;
.
strat:top
  a owl:ObjectProperty ;
  dcterms:description "Boundary of top of unit"@en ;
  rdfs:comment "Boundary of top of unit"@en ;
  rdfs:domain strat:Unit ;
  rdfs:label "top boundary"@en ;
  rdfs:range strat:Boundary ;
  rdfs:subPropertyOf strat:relation ;
.
strat:topAge
  a owl:ObjectProperty ;
  dcterms:description "Age of top of unit"@en ;
  rdfs:comment "Age of top of unit"@en ;
  rdfs:domain strat:Unit ;
  rdfs:label "Age of top"@en ;
  rdfs:subPropertyOf strat:age ;
  owl:propertyChainAxiom (
      strat:top
      strat:age
    ) ;
  skos:example """
stratnames:u27732
  rdf:type strat:Unit ;
  strat:topAge <http://resource.geosciml.org/classifier/ics/ischart/Pleistocene> ;
.
""" ;
.
strat:wasDefinedBy
  a owl:ObjectProperty ;
  dcterms:description "was defined by"@en ;
  rdfs:comment "was defined by"@en ;
  rdfs:range <http://www.w3.org/ns/prov#Agent> ;
  rdfs:subPropertyOf <http://www.w3.org/ns/prov#wasAttributedTo> ;
  skos:example """
stratnames:u27732
  rdf:type strat:Unit ;
  strat:wasDefinedBy <https://orcid.org/0000-1111-2222-3333> ;
.
""" ;
.
strat:within
  a owl:ObjectProperty ;
  rdfs:label "is within "@en ;
  rdfs:subPropertyOf dcterms:relation ;
.
lith:acid_igneous_rock
  a strat:Lithology-group ;
  a owl:NamedIndividual ;
  rdfs:label "acid igneous rock" ;
.
lith:acid_intrusive_rock
  a strat:Lithology-group ;
  a owl:NamedIndividual ;
  rdfs:label "acid intrusive rock" ;
.
lith:acid_volcanic_rock
  a strat:Lithology-group ;
  a owl:NamedIndividual ;
  rdfs:label "acid volcanic rock" ;
  rdfs:label "acid volcanic rock"@en ;
.
lith:basic_igneous_rock
  a strat:Lithology-group ;
  a owl:NamedIndividual ;
  rdfs:label "basic igneous rock" ;
.
lith:basic_intrusive_rock
  a strat:Lithology-group ;
  a owl:NamedIndividual ;
  rdfs:label "basic intrusive rock" ;
.
lith:basic_volcanic_rock
  a strat:Lithology-group ;
  a owl:NamedIndividual ;
  rdfs:label "basic volcanic rock" ;
.
lith:biogenic_silica_sedimentary_rock
  a strat:Lithology-group ;
  a owl:NamedIndividual ;
  rdfs:label "biogenic silica sedimentary rock" ;
.
lith:carbonate_sedimentary_rock
  a strat:Lithology-group ;
  a owl:NamedIndividual ;
  rdfs:label "carbonate sedimentary rock" ;
.
lith:exotic_composition_igneous_rock
  a strat:Lithology-group ;
  a owl:NamedIndividual ;
  rdfs:label "exotic composition igneous rock" ;
.
lith:fine_grained_siliciclastic_rock
  a strat:Lithology-group ;
  a owl:NamedIndividual ;
  rdfs:label "fine grained siliciclastic rock" ;
.
lith:high_grade_metamorphic_rock
  a strat:Lithology-group ;
  a owl:NamedIndividual ;
  rdfs:label "high grade metamorphic rock" ;
.
lith:igneous_intrusive_rock
  a strat:Lithology-group ;
  a owl:NamedIndividual ;
  rdfs:label "igneous intrusive rock" ;
.
lith:igneous_rock
  a strat:Lithology-group ;
  a owl:NamedIndividual ;
  rdfs:label "igneous rock" ;
.
lith:igneous_volcanic_rock
  a strat:Lithology-group ;
  a owl:NamedIndividual ;
  rdfs:label "igneous volcanic rock" ;
.
lith:intermediate_intrusive_rock
  a strat:Lithology-group ;
  a owl:NamedIndividual ;
  rdfs:label "intermediate intrusive rock" ;
.
lith:intermediate_volcanic_rock
  a strat:Lithology-group ;
  a owl:NamedIndividual ;
  rdfs:label "intermediate volcanic rock" ;
.
lith:low-intermediate_grade_metamorphic_rock
  a strat:Lithology-group ;
  a owl:NamedIndividual ;
  rdfs:label "low-intermediate grade metamorphic rock" ;
.
lith:medium-coarse_grained_siliciclastic_rock
  a strat:Lithology-group ;
  a owl:NamedIndividual ;
  rdfs:label "medium-coarse grained siliciclastic rock" ;
  rdfs:label "medium-coarse grained siliciclastic rock"@en ;
.
lith:metamorphic_rock
  a strat:Lithology-group ;
  a owl:NamedIndividual ;
  rdfs:label "metamorphic rock" ;
.
lith:metamorphosed_acid_igneous_rock
  a strat:Lithology-group ;
  a owl:NamedIndividual ;
  rdfs:label "metamorphosed acid igneous rock" ;
.
lith:metamorphosed_basic_igneous_rock
  a strat:Lithology-group ;
  a owl:NamedIndividual ;
  rdfs:label "metamorphosed basic igneous rock" ;
.
lith:metamorphosed_igneous_rock
  a strat:Lithology-group ;
  a owl:NamedIndividual ;
  rdfs:label "metamorphosed igneous rock" ;
.
lith:metamorphosed_ultramafic_rock
  a strat:Lithology-group ;
  a owl:NamedIndividual ;
  rdfs:label "metamorphosed ultramafic rock" ;
.
lith:metasedimentary_carbonate_rock
  a strat:Lithology-group ;
  a owl:NamedIndividual ;
  rdfs:label "metasedimentary carbonate rock" ;
.
lith:metasedimentary_non-carbonate_chemical_or_biochemical_rock
  a strat:Lithology-group ;
  a owl:NamedIndividual ;
  rdfs:label "metasedimentary non-carbonate chemical or biochemical rock" ;
.
lith:metasedimentary_rock
  a strat:Lithology-group ;
  a owl:NamedIndividual ;
  rdfs:label "metasedimentary rock" ;
.
lith:metasedimentary_siliciclastic_rock
  a strat:Lithology-group ;
  a owl:NamedIndividual ;
  rdfs:label "metasedimentary siliciclastic rock" ;
.
lith:mineralisation
  a strat:Lithology-group ;
  a owl:NamedIndividual ;
  rdfs:label "mineralisation" ;
.
lith:non-carbonate_chemical_or_biochemical_sedimentary_rock
  a strat:Lithology-group ;
  a owl:NamedIndividual ;
  rdfs:label "non-carbonate chemical or biochemical sedimentary rock" ;
.
lith:organic_rich_sedimentary_rock
  a strat:Lithology-group ;
  a owl:NamedIndividual ;
  rdfs:label "organic rich sedimentary rock" ;
.
lith:regolith
  a strat:Lithology-group ;
  a owl:NamedIndividual ;
  rdfs:label "regolith" ;
.
lith:sedimentary_rock
  a strat:Lithology-group ;
  a owl:NamedIndividual ;
  rdfs:label "sedimentary rock" ;
.
lith:siliciclastic_sedimentary_rock
  a strat:Lithology-group ;
  a owl:NamedIndividual ;
  rdfs:label "siliciclastic sedimentary rock" ;
.
lith:ultramafic_igneous_rock
  a strat:Lithology-group ;
  a owl:NamedIndividual ;
  rdfs:label "ultramafic igneous rock" ;
.
lith:ultramafic_intrusive_rock
  a strat:Lithology-group ;
  a owl:NamedIndividual ;
  rdfs:label "ultramafic intrusive rock" ;
.
lith:ultramafic_volcanic_rock
  a strat:Lithology-group ;
  a owl:NamedIndividual ;
  rdfs:label "ultramafic volcanic rock" ;
.
proc:alteration
  a strat:Geologic-process ;
  a owl:NamedIndividual ;
  rdfs:Label "alteration" ;
.
proc:deformation
  a strat:Geologic-process ;
  a owl:NamedIndividual ;
  rdfs:Label "deformation" ;
.
proc:deposition
  a strat:Geologic-process ;
  a owl:NamedIndividual ;
  rdfs:Label "deposition" ;
.
proc:diagenesis
  a strat:Geologic-process ;
  a owl:NamedIndividual ;
  rdfs:Label "diagenesis" ;
.
proc:eruption
  a strat:Geologic-process ;
  a owl:NamedIndividual ;
  rdfs:Label "eruption" ;
.
proc:intrusion
  a strat:Geologic-process ;
  a owl:NamedIndividual ;
  rdfs:Label "intrusion" ;
.
proc:magmatic-crystallisation
  a strat:Geologic-process ;
  a owl:NamedIndividual ;
  rdfs:Label "magmatic crystallisation" ;
.
proc:maximum-depositional-age
  a strat:Geologic-process ;
  a owl:NamedIndividual ;
  rdfs:Label "maximum depositional age" ;
.
proc:metamorphism
  a strat:Geologic-process ;
  a owl:NamedIndividual ;
  rdfs:Label "metamorphism" ;
.
proc:minimum-depositional-age
  a strat:Geologic-process ;
  a owl:NamedIndividual ;
  rdfs:Label "minimum depositional age" ;
.
proc:tectonic-process
  a strat:Geologic-process ;
  a owl:NamedIndividual ;
  rdfs:Label "tectonic process" ;
.
proc:weathering
  a strat:Geologic-process ;
  a owl:NamedIndividual ;
  rdfs:Label "weathering" ;
.
rel:abuts
  a strat:Relation-type ;
  a owl:NamedIndividual ;
  rdfs:label "abuts" ;
.
rel:grades-into
  a strat:Relation-type ;
  a owl:NamedIndividual ;
  rdfs:label "grades into" ;
.
rel:hosts
  a strat:Relation-type ;
  a owl:NamedIndividual ;
  rdfs:label "hosts" ;
.
rel:intermingles-with
  a strat:Relation-type ;
  a owl:NamedIndividual ;
  rdfs:label "intermingles with" ;
.
rel:intersects
  a strat:Relation-type ;
  a owl:NamedIndividual ;
  rdfs:label "intersects" ;
.
rel:intrudes
  a strat:Relation-type ;
  a owl:NamedIndividual ;
  rdfs:label "intrudes" ;
.
rel:is-equivalent-to
  a strat:Relation-type ;
  a owl:NamedIndividual ;
  rdfs:label "is equivalent to" ;
.
rel:is-faulted-against
  a strat:Relation-type ;
  a owl:NamedIndividual ;
  rdfs:label "is faulted against" ;
.
rel:is-hosted-by
  a strat:Relation-type ;
  a owl:NamedIndividual ;
  rdfs:label "is hosted by" ;
.
rel:is-interbedded-with
  a strat:Relation-type ;
  a owl:NamedIndividual ;
  rdfs:label "is interbedded with" ;
.
rel:is-intersected-by
  a strat:Relation-type ;
  a owl:NamedIndividual ;
  rdfs:label "is intersected by" ;
.
rel:is-intruded-by
  a strat:Relation-type ;
  a owl:NamedIndividual ;
  rdfs:label "is intruded by" ;
.
rel:is-replaced-by
  a strat:Relation-type ;
  a owl:NamedIndividual ;
  rdfs:label "is replaced by" ;
.
rel:overlies
  a strat:Relation-type ;
  a owl:NamedIndividual ;
  rdfs:label "overlies" ;
.
rel:replaces
  a strat:Relation-type ;
  a owl:NamedIndividual ;
  rdfs:label "replaces" ;
.
rel:underlies
  a strat:Relation-type ;
  a owl:NamedIndividual ;
  rdfs:label "underlies" ;
.
rel:unknown
  a strat:Relation-type ;
  a owl:NamedIndividual ;
  rdfs:label "unknown" ;
.
<http://resource.geosciml.org/ontology/timescale/gts#GeochronologicBoundary>
  rdfs:subClassOf [
      a owl:Restriction ;
      owl:allValuesFrom <http://resource.geosciml.org/ontology/timescale/gts#StratigraphicPoint> ;
      owl:onProperty <http://resource.geosciml.org/ontology/timescale/gts#stratotype> ;
    ] ;
.
<http://resource.geosciml.org/ontology/timescale/gts#GeochronologicEra>
  rdfs:subClassOf [
      a owl:Restriction ;
      owl:allValuesFrom <http://resource.geosciml.org/ontology/timescale/gts#StratigraphicSection> ;
      owl:onProperty <http://resource.geosciml.org/ontology/timescale/gts#stratotype> ;
    ] ;
.
<http://resource.geosciml.org/ontology/timescale/gts#StratigraphicSection>
  rdfs:subClassOf strat:Section ;
.
<http://resource.geosciml.org/ontology/timescale/gts#stratotype>
  rdfs:domain [
      a owl:Class ;
      owl:unionOf (
          <http://resource.geosciml.org/ontology/timescale/gts#GeochronologicBoundary>
          <http://resource.geosciml.org/ontology/timescale/gts#GeochronologicEra>
        ) ;
    ] ;
  rdfs:range [
      a owl:Class ;
      owl:unionOf (
          <http://resource.geosciml.org/ontology/timescale/gts#StratigraphicPoint>
          <http://resource.geosciml.org/ontology/timescale/gts#StratigraphicSection>
        ) ;
    ] ;
  rdfs:subPropertyOf strat:manifestedBy ;
.
<http://resource.geosciml.org/ontology/timescale/rank/Age>
  a owl:NamedIndividual ;
.
<http://resource.geosciml.org/ontology/timescale/rank/Eon>
  a owl:NamedIndividual ;
.
<http://resource.geosciml.org/ontology/timescale/rank/Epoch>
  a owl:NamedIndividual ;
.
<http://resource.geosciml.org/ontology/timescale/rank/Era>
  a owl:NamedIndividual ;
.
<http://resource.geosciml.org/ontology/timescale/rank/Period>
  a owl:NamedIndividual ;
.
<http://resource.geosciml.org/ontology/timescale/rank/Sub-Period>
  a owl:NamedIndividual ;
.
<http://resource.geosciml.org/ontology/timescale/rank/Super-Eon>
  a owl:NamedIndividual ;
.
geo:sfContains
  rdfs:subPropertyOf strat:contains ;
.
geo:sfWithin
  rdfs:subPropertyOf strat:within ;
.
